src/TrsInv.v
@@ -5,60 +5,45 @@ Require Import Simulation Serial.
 Set Implicit Arguments.
 
 Definition OInv := OState -> Prop.
-Definition Inv := TState -> Prop.
+Definition TInv := TState -> Prop.
 
-Definition liftOInv (oidx: IdxT) (oinv: OInv): Inv :=
+Definition liftOInv (oidx: IdxT) (oinv: OInv): TInv :=
   fun tst => (tst_oss tst)@[oidx] >>=[True] (fun ost => oinv ost).
 
-Definition invAnd (inv1 inv2: Inv) :=
+Definition tInvAnd (inv1 inv2: TInv) :=
   fun tst => inv1 tst /\ inv2 tst.
-Infix "/\i" := invAnd (at level 80).
+Infix "/\i" := tInvAnd (at level 80).
 
-Definition invImp (inv1 inv2: Inv) :=
+Definition tInvImp (inv1 inv2: TInv) :=
   forall tst, inv1 tst -> inv2 tst.
-Infix "->i" := invImp (at level 99).
+Infix "->i" := tInvImp (at level 99).
 
-Lemma inv_proj1: forall inv1 inv2, inv1 /\i inv2 ->i inv1.
+Lemma tinv_proj1: forall inv1 inv2, inv1 /\i inv2 ->i inv1.
 Proof. firstorder. Qed.
-Lemma inv_proj2: forall inv1 inv2, inv1 /\i inv2 ->i inv2.
-Proof. firstorder. Qed.
-
-Definition AInv := TrsId -> Msg -> THistory -> MessagePool TMsg -> TState -> Prop.
-Definition ainvAnd (ainv1 ainv2: AInv) :=
-  fun ts rq hst mouts tst =>
-    ainv1 ts rq hst mouts tst /\ ainv2 ts rq hst mouts tst.
-Infix "/\a" := ainvAnd (at level 80).
-Definition ainvImp (ainv1 ainv2: AInv) :=
-  forall ts rq hst mouts tst,
-    ainv1 ts rq hst mouts tst -> ainv2 ts rq hst mouts tst.
-Infix "->a" := ainvImp (at level 99).
-
-Lemma ainv_proj1: forall ainv1 ainv2, ainv1 /\a ainv2 ->a ainv1.
-Proof. firstorder. Qed.
-Lemma ainv_proj2: forall ainv1 ainv2, ainv1 /\a ainv2 ->a ainv2.
+Lemma tinv_proj2: forall inv1 inv2, inv1 /\i inv2 ->i inv2.
 Proof. firstorder. Qed.
 
 Section Impl.
   Variable (impl: System).
 
-  Definition TrsInvInit (ginv: Inv) :=
+  Definition TrsInvInit (ginv: TInv) :=
     ginv (initsOf impl).
 
-  Definition TrsInv (ginv: Inv) :=
+  Definition TrsInv (ginv: TInv) :=
     forall ist1,
       ginv ist1 ->
       forall ihst ist2,
         trsSteps impl ist1 ihst ist2 ->
         ginv ist2.
 
-  Definition TrsInvIn (ginv: Inv) :=
+  Definition TrsInvIn (ginv: TInv) :=
     forall ist1,
       ginv ist1 ->
       forall imin ist2,
         step_det impl ist1 (RlblIn imin) ist2 ->
         ginv ist2.
 
-  Definition TrsInvAtomic (ginv: Inv) :=
+  Definition TrsInvAtomic (ginv: TInv) :=
     forall ts rq hst mouts,
       Atomic impl ts rq hst mouts ->
       forall ist1,
@@ -66,14 +51,6 @@ Section Impl.
         forall ist2,
           steps_det impl ist1 hst ist2 ->
           ginv ist2.
-
-  Definition TrsAInv (ginv: Inv) (ainv: AInv) :=
-    forall ts rq hst mouts,
-      Atomic impl ts rq hst mouts ->
-      forall ist1 ist2,
-        steps_det impl ist1 hst ist2 ->
-        ginv ist1 ->
-        ainv ts rq hst mouts ist2.
 
 End Impl.
 
@@ -83,29 +60,8 @@ Lemma trsInv_split:
     TrsInv impl inv2 ->
     TrsInv impl (inv1 /\i inv2).
 Proof.
-  unfold TrsInv, invAnd; intros; dest; split; eauto.
+  unfold TrsInv, tInvAnd; intros; dest; split; eauto.
 Qed.
 
 Ltac split_inv := apply trsInv_split.
-
-Lemma trsAInv_split:
-  forall impl ginv ainv1 ainv2,
-    TrsAInv impl ginv ainv1 ->
-    TrsAInv impl ginv ainv2 ->
-    TrsAInv impl ginv (ainv1 /\a ainv2).
-Proof.
-  intros; split; eauto.
-Qed.
-
-Ltac split_ainv := apply trsAInv_split.
-
-Lemma trsAInv_ginv_weaken:
-  forall impl ginv1 ainv,
-    TrsAInv impl ginv1 ainv ->
-    forall ginv2,
-      ginv2 ->i ginv1 ->
-      TrsAInv impl ginv2 ainv.
-Proof.
-  unfold TrsAInv; intros; eauto.
-Qed.
 
