src/StepDet.v
@@ -13,20 +13,16 @@ Fixpoint getTMsgsTInfo (tmsgs: list TMsg) :=
 
 Inductive step_det (sys: System): TState -> TLabel -> TState -> Prop :=
 | SdSlt: forall st, step_det sys st emptyRLabel st
-| SdExt: forall ts oss oims emsg,
+| SdExt: forall ts pst nst oss oims emsg,
     isExternal sys (mid_from (msg_id emsg)) = true ->
     isInternal sys (mid_to (msg_id emsg)) = true ->
-    step_det sys
-             {| tst_oss := oss;
-                tst_msgs := oims;
-                tst_tid := ts
-             |}
-             (RlblIn (toTMsgU emsg))
-             {| tst_oss := oss;
-                tst_msgs := enqMP (toTMsgU emsg) oims;
-                tst_tid := ts
-             |}
-| SdInt: forall ts nts (Hts: nts > ts) tinfo
+    pst = {| tst_oss := oss; tst_msgs := oims; tst_tid := ts |} ->
+    nst = {| tst_oss := oss;
+             tst_msgs := enqMP (toTMsgU emsg) oims;
+             tst_tid := ts
+          |} ->
+    step_det sys pst (RlblIn (toTMsgU emsg)) nst
+| SdInt: forall ts pst nst nts (Hts: nts > ts) tinfo
                 oss oims oidx os pos msgs rule outs,
     In oidx (indicesOf sys) ->
     (oss)@[oidx] = Some os ->
@@ -43,21 +39,18 @@ Inductive step_det (sys: System): TState -> TLabel -> TState -> Prop :=
             | None => {| tinfo_tid := nts; tinfo_rqin := map tmsg_msg msgs |}
             end ->
 
-    step_det sys
-             {| tst_oss := oss;
-                tst_msgs := oims;
-                tst_tid := ts
-             |}
-             (RlblOuts (Some rule) msgs (toTMsgs tinfo outs))
-             {| tst_oss := oss +[ oidx <- pos ];
-                tst_msgs := distributeMsgs
-                              (intOuts sys (toTMsgs tinfo outs))
-                              (removeMsgs msgs oims);
-                tst_tid := match getTMsgsTInfo msgs with
-                           | Some _ => ts
-                           | None => nts
-                           end
-             |}.
+    pst = {| tst_oss := oss; tst_msgs := oims; tst_tid := ts |} ->
+    nst = {| tst_oss := oss +[ oidx <- pos ];
+             tst_msgs := distributeMsgs
+                           (intOuts sys (toTMsgs tinfo outs))
+                           (removeMsgs msgs oims);
+             tst_tid := match getTMsgsTInfo msgs with
+                        | Some _ => ts
+                        | None => nts
+                        end
+          |} ->
+
+    step_det sys pst (RlblOuts (Some rule) msgs (toTMsgs tinfo outs)) nst.
 
 Definition steps_det: Steps System TState TLabel := steps step_det.
 
